proj1/src/SeqAndSet.dfy
@@ -1,0 +1,84 @@
+/**
+    Helper functions and lemmas about conversion between set and seq.
+ */
+
+module SeqAndSet {
+  lemma seq2setAdd(s: seq<nat>, k: nat)
+  ensures seq2set(s + [k]) == seq2set(s) + {k}
+  {
+    if s == [] {
+    } else {
+      calc {
+            seq2set(s + [k]);
+          == { assert s == [s[0]] + s[1..]; }
+            seq2set(([s[0]] + s[1..]) + [k]);
+          == { assert ([s[0]] + s[1..]) + [k] == [s[0]] + (s[1..] + [k]);}
+            seq2set([s[0]] + (s[1..] + [k]));
+          ==
+            seq2set(s) + {k};
+      }
+    }
+  }
+
+  lemma seq2seqEquiv(s: seq<nat>, c: set<nat>, k: nat)
+    requires c == seq2set(s)
+
+    ensures k in c <==> k in s
+  {
+    if k in c {
+      seq2seqEquivAux(s, c, k);
+      assert k in s;
+
+    } else {
+      if k in s {
+          // contradiction
+          seq2seqEquivAux2(s, c, k);
+          assert k in c;
+      } else {
+
+      }
+    }
+  }
+
+  lemma seq2seqEquivAux(s: seq<nat>, c: set<nat>, k: nat)
+    requires c == seq2set(s)
+    requires k in c
+    
+    ensures k in s
+  {
+    if s == [] {
+    } else {
+      if k == s[0] {
+      } else {
+        seq2seqEquivAux(s[1..], seq2set(s[1..]), k);
+      }
+    }
+
+  }
+
+  lemma seq2seqEquivAux2(s: seq<nat>, c: set<nat>, k: nat)
+    requires c == seq2set(s)
+    requires k in s
+    
+    ensures k in c
+  {
+    if s[0] == k {
+    } else {
+      seq2seqEquivAux2(s[1..], seq2set(s[1..]), k);
+    }
+  }
+
+  lemma seq2setGood(s1: seq<nat>, s2: seq<nat>)
+    requires s1 == s2
+    ensures seq2set(s1) == seq2set(s2)
+  {
+  }
+
+  /**
+    Converts seq to set
+   */
+  function seq2set(s: seq<nat>): set<nat>
+  {
+    if s == [] then {} else {s[0]} + seq2set(s[1..])
+  }
+}
